changed the standard sts with two new states for monotone invariants, and added a new kind of transition to the standard sts. Updated the logical relation accordingly

theories/logrel.v
@@ -87,26 +87,27 @@ Section logrel.
     solve_proper.
   Qed.
 
-  Definition future_world g W W' : iProp Σ :=
+  Definition future_world g l W W' : iProp Σ :=
     (match g with
-    | Local => ⌜related_sts_pub_world W W'⌝
+    | Local => ⌜related_sts_pub_plus_world W W'⌝
     | Global => ⌜related_sts_priv_world W W'⌝
+    | Monotone => ⌜related_sts_a_world W W' l⌝
      end)%I.
 
-  Global Instance future_world_persistent g W W': Persistent (future_world g W W').
+  Global Instance future_world_persistent g l W W': Persistent (future_world g l W W').
   Proof.
     unfold future_world. destruct g; apply bi.pure_persistent.
   Qed.
 
   Definition exec_cond W b e g p (interp : D) : iProp Σ :=
-    (∀ a r W', ⌜a ∈ₐ [[ b , e ]]⌝ → future_world g W W' →
+    (∀ a r W', ⌜a ∈ₐ [[ b , e ]]⌝ → future_world g e W W' →
             ▷ interp_expr interp r W' (inr ((p,g),b, e,a)))%I.
   Global Instance exec_cond_ne n :
     Proper ((=) ==> (=) ==> (=) ==> (=) ==> (=) ==> dist n ==> dist n) exec_cond.
   Proof. unfold exec_cond. solve_proper. Qed.
 
   Definition enter_cond W b e a g (interp : D) : iProp Σ :=
-    (∀ r W', future_world g W W' →
+    (∀ r W', future_world g e W W' →
         ▷ interp_expr interp r W' (inr ((RX,g),b,e,a)))%I.
   Global Instance enter_cond_ne n :
     Proper ((=) ==> (=) ==> (=) ==> (=) ==> (=) ==> dist n ==> dist n) enter_cond.
@@ -117,14 +118,34 @@ Section logrel.
 
   Definition interp_cap_O : D := λne _ _, True%I.
 
+  (*
+      -------------------------------------------------------------
+      |          |         nwl           |          pwl           |
+      |          | - < a    |    a ≤ -   |  - < a    |    a ≤ -   |
+      -------------------------------------------------------------
+      | Monotone | {M,T,P} | {M,T,P,MF,F}|    {M}    |    {M,MF}  |
+      |-----------------------------------------------------------|
+      | Local    | {T,P}   | {T,P,F}     |    {T}    |    {T,F}   |
+      |-----------------------------------------------------------|
+      | Global   |        {P}            |           N/A          |
+      -------------------------------------------------------------
+
+   *)
+
   Definition region_state_pwl W (a : Addr) : Prop :=
     (std W) !! a = Some Temporary.
+
+  Definition region_state_pwl_mono W (a : Addr) : Prop :=
+    (std W) !! a = Some Monotemporary.
 
   Definition region_state_nwl W (a : Addr) (l : Locality) : Prop :=
     match l with
      | Local => (std W) !! a = Some Temporary
                ∨ (std W) !! a = Some Permanent
-    | Global => (std W) !! a = Some Permanent
+     | Global => (std W) !! a = Some Permanent
+     | Monotone => (std W) !! a = Some Monotemporary
+                  ∨ (std W) !! a = Some Temporary
+                  ∨ (std W) !! a = Some Permanent
     end.
 
   Definition region_state_U W (a : Addr) : Prop :=
@@ -132,9 +153,21 @@ Section logrel.
     \/ (std W) !! a = Some Permanent
     ∨ (exists w, (std W) !! a = Some (Static {[a:=w]})).
 
+  Definition region_state_U_mono W (a : Addr) : Prop :=
+    (std W) !! a = Some Monotemporary
+    ∨ (std W) !! a = Some Temporary
+    \/ (std W) !! a = Some Permanent
+    ∨ (exists w, (std W) !! a = Some (Static {[a:=w]}))
+    ∨ (exists w, (std W) !! a = Some (Monostatic {[a:=w]})).
+
   Definition region_state_U_pwl W (a : Addr) : Prop :=
     (std W) !! a = Some Temporary
     ∨ (exists w, (std W) !! a = Some (Static {[a:=w]})).
+
+  Definition region_state_U_pwl_mono W (a : Addr) : Prop :=
+    (std W) !! a = Some Monotemporary
+    ∨ (exists w, (std W) !! a = Some (Monostatic {[a:=w]})).
+
 
   (* For simplicity we might want to have the following statement in valididy of caps. However, it is strictly not
      necessary since it can be derived form full_sts_world *)
@@ -159,17 +192,19 @@ Section logrel.
 
   Program Definition interp_cap_RWL (interp : D) : D :=
     λne W w, (match w with
+              | inr ((RWL,Monotone),b,e,a) =>
+                [∗ list] a ∈ (region_addrs b e), ∃ p, ⌜PermFlows RWL p⌝ ∗ (read_write_cond a p interp) ∧ ⌜region_state_pwl_mono W a⌝
               | inr ((RWL,Local),b,e,a) =>
-                      [∗ list] a ∈ (region_addrs b e), ∃ p, ⌜PermFlows RWL p⌝ ∗ (read_write_cond a p interp) ∧ ⌜region_state_pwl W a⌝
+                [∗ list] a ∈ (region_addrs b e), ∃ p, ⌜PermFlows RWL p⌝ ∗ (read_write_cond a p interp) ∧ ⌜region_state_pwl W a⌝
               | _ => False
               end)%I.
-  Solve All Obligations with solve_proper.
+  Solve All Obligations with solve_proper;auto.
 
   Program Definition interp_cap_RX (interp : D) : D :=
-    λne W w, (match w with inr ((RX,g),b,e,a) =>
-                           ([∗ list] a ∈ (region_addrs b e), ∃ p, ⌜PermFlows RX p⌝ ∗ (read_write_cond a p interp)
-                                                                   ∧ ⌜region_state_nwl W a g⌝)
-                                 (* ∗ □ exec_cond W b e g RX interp *)
+    λne W w, (match w with
+              | inr ((RX,g),b,e,a) =>
+                ([∗ list] a ∈ (region_addrs b e), ∃ p, ⌜PermFlows RX p⌝ ∗ (read_write_cond a p interp)
+                                                       ∧ ⌜region_state_nwl W a g⌝)
              | _ => False end)%I.
   Solve All Obligations with solve_proper.
 
@@ -181,23 +216,32 @@ Section logrel.
   Solve All Obligations with solve_proper.
 
   Program Definition interp_cap_RWX (interp : D) : D :=
-    λne W w, (match w with inr ((RWX,g),b,e,a) =>
-                           ([∗ list] a ∈ (region_addrs b e), ∃ p, ⌜PermFlows RWX p⌝ ∗ (read_write_cond a p interp)
-                                                                   ∧ ⌜region_state_nwl W a g⌝)
-                                 (* ∗ □ exec_cond W b e g RWX interp *)
-             | _ => False end)%I.
+    λne W w, (match w with
+              | inr ((RWX,g),b,e,a) =>
+                ([∗ list] a ∈ (region_addrs b e), ∃ p, ⌜PermFlows RWX p⌝ ∗ (read_write_cond a p interp)
+                                                       ∧ ⌜region_state_nwl W a g⌝)
+              | _ => False end)%I.
   Solve All Obligations with solve_proper.
 
   Program Definition interp_cap_RWLX (interp : D) : D :=
-    λne W w, (match w with inr ((RWLX,Local),b,e,a) =>
-                           ([∗ list] a ∈ (region_addrs b e), ∃ p, ⌜PermFlows RWLX p⌝ ∗ (read_write_cond a p interp)
-                                                                   ∧ ⌜region_state_pwl W a⌝)
-                                 (* ∗ □ exec_cond W b e Local RWLX interp *)
-             | _ => False end)%I.
+    λne W w, (match w with
+              | inr ((RWLX,Monotone),b,e,a) =>
+                ([∗ list] a ∈ (region_addrs b e), ∃ p, ⌜PermFlows RWLX p⌝ ∗ (read_write_cond a p interp)
+                                                       ∧ ⌜region_state_pwl_mono W a⌝)
+              | inr ((RWLX,Local),b,e,a) =>
+                ([∗ list] a ∈ (region_addrs b e), ∃ p, ⌜PermFlows RWLX p⌝ ∗ (read_write_cond a p interp)
+                                                       ∧ ⌜region_state_pwl W a⌝)
+              | _ => False end)%I.
   Solve All Obligations with solve_proper.
-
+  
   Program Definition interp_cap_URW (interp : D) : D :=
     λne W w, (match w with
+              | inr ((URW,Monotone),b,e,a) =>
+                ([∗ list] a' ∈ (region_addrs b (addr_reg.min a e)), ∃ p, ⌜PermFlows (promote_perm URW) p⌝
+                                                                          ∗ (read_write_cond a' p interp)
+                                                                         ∧ ⌜region_state_nwl W a' Monotone⌝) ∗
+                                             ([∗ list] a' ∈ (region_addrs (addr_reg.max b a) e), ∃ p, ⌜PermFlows (promote_perm URW) p⌝
+                                                                                                                                                                    ∗ (read_write_cond a' p interp) ∧ ⌜region_state_U_mono W a'⌝)
               | inr ((URW,Local),b,e,a) =>
                 ([∗ list] a' ∈ (region_addrs b (addr_reg.min a e)), ∃ p, ⌜PermFlows (promote_perm URW) p⌝ ∗ (read_write_cond a' p interp)
                                                                  ∧ ⌜region_state_nwl W a' Local⌝) ∗
@@ -210,6 +254,11 @@ Section logrel.
 
   Program Definition interp_cap_URWL (interp : D) : D :=
     λne W w, (match w with
+              | inr ((URWL,Monotone),b,e,a) =>
+                ([∗ list] a' ∈ (region_addrs b (addr_reg.min a e)), ∃ p, ⌜PermFlows (promote_perm URWL) p⌝ ∗ (read_write_cond a' p interp)
+                                                                 ∧ ⌜region_state_pwl_mono W a'⌝) ∗
+                ([∗ list] a' ∈ (region_addrs (addr_reg.max b a) e), ∃ p, ⌜PermFlows (promote_perm URWL) p⌝ ∗ (read_write_cond a' p interp) ∧
+                                                                 ⌜region_state_U_pwl_mono W a'⌝)
               | inr ((URWL,Local),b,e,a) =>
                 ([∗ list] a' ∈ (region_addrs b (addr_reg.min a e)), ∃ p, ⌜PermFlows (promote_perm URWL) p⌝ ∗ (read_write_cond a' p interp)
                                                                  ∧ ⌜region_state_pwl W a'⌝) ∗
@@ -221,21 +270,29 @@ Section logrel.
 
   Program Definition interp_cap_URWX (interp : D) : D :=
     λne W w, (match w with
+              | inr ((URWX,Monotone),b,e,a) =>
+                ([∗ list] a' ∈ (region_addrs b (addr_reg.min a e)), ∃ p, ⌜PermFlows (promote_perm URWX) p⌝ ∗ (read_write_cond a' p interp)
+                                                                 ∧ ⌜region_state_nwl W a' Monotone⌝)
+               ∗ ([∗ list] a' ∈ (region_addrs (addr_reg.max b a) e), ∃ p, ⌜PermFlows (promote_perm URWX) p⌝ ∗ (read_write_cond a' p interp)
+                                                                   ∧ ⌜region_state_U_mono W a'⌝)
               | inr ((URWX,Local),b,e,a) =>
                 ([∗ list] a' ∈ (region_addrs b (addr_reg.min a e)), ∃ p, ⌜PermFlows (promote_perm URWX) p⌝ ∗ (read_write_cond a' p interp)
                                                                  ∧ ⌜region_state_nwl W a' Local⌝)
-                      (* ∗ □ exec_cond W b (addr_reg.min a e) Local RWX interp *)
                ∗ ([∗ list] a' ∈ (region_addrs (addr_reg.max b a) e), ∃ p, ⌜PermFlows (promote_perm URWX) p⌝ ∗ (read_write_cond a' p interp)
                                                                    ∧ ⌜region_state_U W a'⌝)
               | inr ((URWX,Global),b,e,a) =>
                 ([∗ list] a' ∈ (region_addrs b e), ∃ p, ⌜PermFlows (promote_perm URWX) p⌝ ∗ (read_write_cond a' p interp)
                                                                  ∧ ⌜region_state_nwl W a' Global⌝)
-                      (* ∗ □ exec_cond W b e Global RWX interp *)
              | _ => False end)%I.
   Solve All Obligations with solve_proper;auto.
 
   Program Definition interp_cap_URWLX (interp : D) : D :=
     λne W w, (match w with
+              | inr ((URWLX,Monotone),b,e,a) =>
+                ([∗ list] a' ∈ (region_addrs b (addr_reg.min a e)), ∃ p, ⌜PermFlows (promote_perm URWLX) p⌝ ∗ (read_write_cond a' p interp)
+                                                                 ∧ ⌜region_state_pwl_mono W a'⌝)
+                ∗ ([∗ list] a' ∈ (region_addrs (addr_reg.max b a) e), ∃ p, ⌜PermFlows (promote_perm URWLX) p⌝ ∗ (read_write_cond a' p interp) ∧
+                                                                   ⌜region_state_U_pwl_mono W a'⌝)
               | inr ((URWLX,Local),b,e,a) =>
                 ([∗ list] a' ∈ (region_addrs b (addr_reg.min a e)), ∃ p, ⌜PermFlows (promote_perm URWLX) p⌝ ∗ (read_write_cond a' p interp)
                                                                  ∧ ⌜region_state_pwl W a'⌝)
@@ -296,6 +353,12 @@ Section logrel.
     Contractive (interp_cap_RWL).
   Proof. solve_proper_prepare.
          destruct x1; auto. destruct c, p, p, p, p, l; auto.
+         apply big_opL_ne; auto. rewrite /pointwise_relation; intros.
+         apply exist_ne. rewrite /pointwise_relation; intros.
+         apply sep_ne; auto.
+         rewrite /read_write_cond rel_eq /rel_def /saved_pred_own.
+         apply and_ne;auto. apply exist_ne =>γ. apply sep_ne; auto.
+         simpl. f_equiv. solve_contractive.
          apply big_opL_ne; auto. rewrite /pointwise_relation; intros.
          apply exist_ne. rewrite /pointwise_relation; intros.
          apply sep_ne; auto.
@@ -364,8 +427,12 @@ Section logrel.
       apply sep_ne; auto. (* apply sep_ne. *)
       apply and_ne;auto. apply exist_ne =>γ. apply sep_ne; auto.
       simpl. f_equiv. solve_contractive.
-    (* - solve_proper_prepare. *)
-    (*   by apply affinely_ne; apply persistently_ne; apply exec_cond_contractive. *)
+    - rewrite /read_write_cond rel_eq /rel_def /saved_pred_own.
+      apply big_opL_ne; auto. intros ? ? ?.
+      apply exist_ne. rewrite /pointwise_relation; intros.
+      apply sep_ne; auto. (* apply sep_ne. *)
+      apply and_ne;auto. apply exist_ne =>γ. apply sep_ne; auto.
+      simpl. f_equiv. solve_contractive.
   Qed.
   Global Instance interp_cap_URW_contractive :
     Contractive (interp_cap_URW).
@@ -389,11 +456,36 @@ Section logrel.
            apply sep_ne; auto.
            apply and_ne; auto. apply exist_ne => γ. apply sep_ne; auto.
            simpl. f_equiv. solve_contractive.
+         - apply sep_ne; auto.
+           apply big_opL_ne; auto; rewrite /pointwise_relation; intros.
+           apply exist_ne. rewrite /pointwise_relation; intros.
+           apply sep_ne; auto.
+           rewrite /read_write_cond rel_eq /rel_def /saved_pred_own.
+           apply and_ne;auto. apply exist_ne =>γ. apply sep_ne; auto.
+           simpl. f_equiv. solve_contractive.
+           apply big_opL_ne; auto. rewrite /pointwise_relation; intros.
+           rewrite /read_write_cond rel_eq /rel_def /saved_pred_own.
+           apply exist_ne. rewrite /pointwise_relation; intros.
+           apply sep_ne; auto.
+           apply and_ne; auto. apply exist_ne => γ. apply sep_ne; auto.
+           simpl. f_equiv. solve_contractive.
   Qed.
   Global Instance interp_cap_URWL_contractive :
     Contractive (interp_cap_URWL).
   Proof. solve_proper_prepare.
          destruct x1; auto. destruct_cap c. destruct c; auto. destruct c3; auto.
+         apply sep_ne; auto.
+         apply big_opL_ne; auto. rewrite /pointwise_relation; intros.
+         apply exist_ne. rewrite /pointwise_relation; intros.
+         apply sep_ne; auto. rewrite /read_write_cond rel_eq /rel_def /saved_pred_own.
+         apply and_ne;auto. apply exist_ne =>γ. apply sep_ne; auto.
+         simpl. f_equiv. solve_contractive.
+         apply big_opL_ne; auto. rewrite /pointwise_relation; intros.
+         rewrite /read_write_cond rel_eq /rel_def /saved_pred_own.
+         apply exist_ne. rewrite /pointwise_relation; intros.
+         apply sep_ne; auto.
+         apply and_ne; auto. apply exist_ne => γ. apply sep_ne; auto.
+         simpl. f_equiv. solve_contractive.
          apply sep_ne; auto.
          apply big_opL_ne; auto. rewrite /pointwise_relation; intros.
          apply exist_ne. rewrite /pointwise_relation; intros.
@@ -432,14 +524,39 @@ Section logrel.
         rewrite /read_write_cond rel_eq /rel_def /saved_pred_own.
         apply and_ne; auto. apply exist_ne => γ. apply sep_ne; auto.
         simpl. f_equiv. solve_contractive.
+    - apply sep_ne; auto.
+      + apply big_opL_ne; auto. rewrite /pointwise_relation; intros.
+        apply exist_ne. rewrite /pointwise_relation; intros.
+        apply sep_ne; auto.
+        rewrite /read_write_cond rel_eq /rel_def /saved_pred_own.
+        apply and_ne; auto. apply exist_ne =>γ. apply sep_ne; auto.
+        simpl. f_equiv. solve_contractive.
+      + apply big_opL_ne; auto. rewrite /pointwise_relation; intros.
+        apply exist_ne. rewrite /pointwise_relation; intros.
+        apply sep_ne; auto.
+        rewrite /read_write_cond rel_eq /rel_def /saved_pred_own.
+        apply and_ne; auto. apply exist_ne => γ. apply sep_ne; auto.
+        simpl. f_equiv. solve_contractive.
   Qed.
   Global Instance interp_cap_URWLX_contractive :
     Contractive (interp_cap_URWLX).
   Proof.
     rewrite /interp_cap_URWLX.
     solve_proper_prepare.
-    destruct x1; auto. destruct_cap c; destruct c; auto. destruct c3; auto.
+    destruct x1; auto. destruct_cap c; destruct c; auto. destruct c3; auto;
     apply sep_ne.
+    - rewrite /read_write_cond rel_eq /rel_def /saved_pred_own.
+      apply big_opL_ne; auto. intros ? ? ?.
+      apply exist_ne. rewrite /pointwise_relation; intros.
+      apply sep_ne; auto.
+      apply and_ne;auto. apply exist_ne =>γ. apply sep_ne; auto.
+      simpl. f_equiv. solve_contractive.
+    - apply big_opL_ne; auto. rewrite /pointwise_relation; intros.
+      apply exist_ne. rewrite /pointwise_relation; intros.
+      apply sep_ne; auto.
+      rewrite /read_write_cond rel_eq /rel_def /saved_pred_own.
+      apply and_ne; auto. apply exist_ne => γ. apply sep_ne; auto.
+      simpl. f_equiv. solve_contractive.
     - rewrite /read_write_cond rel_eq /rel_def /saved_pred_own.
       apply big_opL_ne; auto. intros ? ? ?.
       apply exist_ne. rewrite /pointwise_relation; intros.
@@ -511,7 +628,7 @@ Section logrel.
     try (iDestruct (extract_from_region_inv with "Hinterp") as (p Hflows) "[Hinv _]"; [eauto|iExists _;iSplit;eauto]).
     - done.
     - done.
-  Qed.
+  Qed. 
 
   Lemma writeLocalAllowed_implies_local W p l b e a:
     pwl p = true ->
@@ -519,40 +636,51 @@ Section logrel.
   Proof.
     intros. iIntros "Hvalid".
     unfold interp; rewrite fixpoint_interp1_eq /=.
-    destruct p; simpl in H; try congruence; destruct l; eauto.
+    destruct p; simpl in H; try congruence; destruct l; eauto. 
   Qed.
 
   Lemma readAllowed_valid_cap_implies W p l b e a:
     readAllowed p = true ->
     withinBounds (p, l, b, e, a) = true ->
     interp W (inr (p, l, b, e, a)) -∗
-           ⌜∃ ρ, std W !! a = Some ρ ∧ ρ <> Revoked ∧ (∀ g, ρ ≠ Static g)⌝.
+           ⌜∃ ρ, std W !! a = Some ρ ∧ ρ <> Revoked ∧ (∀ g, ρ ≠ Static g) ∧ (∀ g, ρ ≠ Monostatic g)⌝.
   Proof.
     intros Hp Hb. iIntros "H".
     eapply withinBounds_le_addr in Hb.
     unfold interp; rewrite fixpoint_interp1_eq /=.
     destruct p; simpl in Hp; try congruence.
     - iDestruct (extract_from_region_inv with "H") as (p ?) "[_ H]"; eauto.
-      iDestruct "H" as %HH. iPureIntro. destruct l; eauto. simpl in HH.
-      destruct HH; eauto.
+      iDestruct "H" as %HH. iPureIntro. destruct l; eauto;simpl in HH.
+      destruct HH;eauto. destruct HH as [? | [? | ?] ]; eauto.
     - iDestruct (extract_from_region_inv with "H") as (p ?) "[_ H]"; eauto.
-      iDestruct "H" as %HH. iPureIntro. destruct l; eauto. simpl in HH.
-      destruct HH; eauto.
+      iDestruct "H" as %HH. iPureIntro. destruct l; eauto; simpl in HH.
+      destruct HH; eauto. destruct HH as [? | [? | ?] ]; eauto.
     - destruct l; auto.
       iDestruct (extract_from_region_inv with "H") as (p ?) "[_ %]"; eauto.
+      iPureIntro. eexists;split;eauto. 
+      iDestruct (extract_from_region_inv with "H") as (p ?) "[_ %]"; eauto.
+      iPureIntro. rewrite H1. eexists;split;eauto. 
     - iDestruct (extract_from_region_inv with "H") as (p ?) "[_ H]"; eauto.
       iDestruct "H" as %HH. iPureIntro. destruct l; eauto. simpl in HH.
-      destruct HH; eauto.
+      destruct HH; eauto. destruct HH;eauto. destruct H1;eauto. 
     - iDestruct (extract_from_region_inv with "H") as (p ?) "[_ H]"; eauto.
       iDestruct "H" as %HH. iPureIntro. destruct l; eauto. simpl in HH.
-      destruct HH; eauto.
+      destruct HH; eauto. destruct HH;eauto. destruct H1;eauto. 
     - destruct l;auto.
       iDestruct (extract_from_region_inv with "H") as (p ?) "[_ %]"; eauto.
+      rewrite H1. iPureIntro. eexists;eauto.
+      iDestruct (extract_from_region_inv with "H") as (p ?) "[_ %]"; eauto.
+      rewrite H1. iPureIntro. eexists;eauto.
   Qed.
 
   Definition region_conditions W p g b e:=
   ([∗ list] a ∈ (region_addrs b e), ∃ p', ⌜PermFlows p p'⌝ ∗ (read_write_cond a p' interp)
-                                             ∧ ⌜if pwl p then region_state_pwl W a else region_state_nwl W a g⌝)%I.
+                                          ∧ ⌜if pwl p
+                                             then (match g with
+                                                   | Monotone => region_state_pwl_mono W a
+                                                   | _ => region_state_pwl W a
+                                                   end)
+                                             else region_state_nwl W a g⌝)%I.
 
   Lemma readAllowed_implies_region_conditions W p l b e a:
     readAllowed p = true ->
@@ -564,12 +692,14 @@ Section logrel.
     destruct p; simpl in *; try congruence; destruct l; simpl; auto.
   Qed.
 
-
   Lemma writeLocalAllowed_valid_cap_implies W p l b e a:
     pwl p = true ->
     withinBounds (p, l, b, e, a) = true ->
     interp W (inr (p, l, b, e, a)) -∗
-           ⌜std W !! a = Some Temporary⌝.
+           ⌜match l with
+            | Monotone => std W !! a = Some Monotemporary
+            | _ => std W !! a = Some Temporary
+            end⌝.
   Proof.
     intros Hp Hb. iIntros "Hvalid".
     iAssert (⌜isLocal l = true⌝)%I as "%". by iApply writeLocalAllowed_implies_local.
@@ -578,7 +708,9 @@ Section logrel.
     destruct p; simpl in Hp; try congruence; destruct l.
     - by exfalso.
     - iDestruct (extract_from_region_inv with "Hvalid") as (? ?) "[_ %]"; eauto.
+    - iDestruct (extract_from_region_inv with "Hvalid") as (? ?) "[_ %]"; eauto.
     - by exfalso.
+    - iDestruct (extract_from_region_inv with "Hvalid") as (? ?) "[_ %]"; eauto.
     - iDestruct (extract_from_region_inv with "Hvalid") as (? ?) "[_ %]"; eauto.
   Qed.
 
@@ -589,11 +721,22 @@ Section logrel.
                ([∗ list] a ∈ region_addrs b (if isU p && isLocal l then (addr_reg.min a e) else e),
                 ∃ p', ⌜PermFlows (promote_perm p) p'⌝ ∗
                  (read_write_cond a p' interp) ∧
-                 ⌜if pwlU p then region_state_pwl W a else region_state_nwl W a l⌝) ∗
-                (*(□ match p with RX | RWX | RWLX => exec_cond W b e l p interp | URWX | URWLX => exec_cond W b (if isLocal l then addr_reg.min a e else e) l (promote_perm p) interp | _ => True end) ∗*)
-                (⌜if pwlU p then l = Local else True⌝) ∗
+                      ⌜if pwlU p then (match l with
+                                       | Monotone => region_state_pwl_mono W a
+                                       | _ => region_state_pwl W a
+                                       end) else region_state_nwl W a l⌝) ∗
+                (⌜if pwlU p then isLocal l else True⌝) ∗
                 (if isU p && isLocal l then [∗ list] a ∈ region_addrs (addr_reg.max b a) e,
-                                            ∃ p', ⌜PermFlows (promote_perm p) p'⌝ ∗ read_write_cond a p' interp ∧ ⌜if pwlU p then region_state_U_pwl W a else region_state_U W a⌝ else emp%I))%I).
+                                            ∃ p', ⌜PermFlows (promote_perm p) p'⌝ ∗ read_write_cond a p' interp ∧
+                                                  ⌜if pwlU p
+                                                   then (match l with
+                                                         | Monotone => region_state_U_pwl_mono W a
+                                                         | _ => region_state_U_pwl W a
+                                                         end)
+                                                   else (match l with
+                                                         | Monotone => region_state_U_mono W a
+                                                         | _ => region_state_U W a
+                                                         end)⌝ else emp%I))%I).
   Proof.
     iSplit.
     { iIntros "HA".
@@ -602,8 +745,12 @@ Section logrel.
       destruct p; simpl; try congruence; auto; destruct l;auto.
       - iDestruct "HA" as "[HA HB]"; eauto.
       - iDestruct "HA" as "[HA HB]"; eauto.
+      - iDestruct "HA" as "[HA HB]"; eauto.
       - iDestruct "HA" as "[Ha HB]"; eauto.
-      - iDestruct "HA" as "[HB HC]"; eauto. }
+      - iDestruct "HA" as "[HB HC]"; eauto.
+      - iDestruct "HA" as "[HA HB]"; eauto.
+      - iDestruct "HA" as "[HA HB]"; eauto.
+      - iDestruct "HA" as "[HA HB]"; eauto. }
     { iIntros "A".
       destruct (perm_eq_dec p O); subst; simpl; auto.
       destruct (perm_eq_dec p E); subst; simpl; auto.
@@ -612,8 +759,3 @@ Section logrel.
   Qed.
 
 End logrel.
-
-(* Notation "𝕍( W )" := (interp W) (at level 70). *)
-(* Notation "𝔼( W )" := (λ r, interp_expression r W). *)
-(* Notation "ℝ( W )" := (interp_registers W). *)
-(* Notation "𝕆( W )" := (interp_conf W.1 W.2).  *)
