theories/sts.v
@@ -17,15 +17,23 @@ Definition STS_std_states (A B : Type) {eqD: EqDecision A} {count: Countable A} 
 
 Definition sts_stateUR := authUR (gmapUR positive (exclR (leibnizO positive))).
 Definition sts_relUR :=
-  authUR (gmapUR positive (agreeR (leibnizO ((positive → positive → Prop) * (positive → positive → Prop))))).
+  authUR (gmapUR positive (agreeR (leibnizO ((positive → positive → Prop) * (positive → positive → Prop) * (positive → positive → Prop))))).
 
 Notation STS_states := (gmap positive positive).
-Notation STS_rels := (gmap positive ((positive → positive → Prop) * (positive → positive → Prop))).
+Notation STS_rels := (gmap positive ((positive → positive → Prop) * (positive → positive → Prop) * (positive → positive → Prop ))).
+
+(** A typeclass for comparable *)
+Class Ord A `{EqDecision A} : Type :=
+  { le_a : relation A;
+    le_a_decision : ∀ a1 a2, Decision (le_a a1 a2);
+    le_a_preorder : PreOrder le_a }.
 
 (** Standard STS. *)
+(** The Standard STS is made up of three relations *)
 Class STS_STD (B : Type) :=
   { Rpub : relation B;
-    Rpriv : relation B;}.
+    Rpriv : relation B;
+    Rpubp : relation B; }.
 
 (** The CMRA for the sts collection. *)
 Class STS_preG A B Σ `{EqDecision A, Countable A} :=
@@ -57,7 +65,9 @@ Qed.
 
 Section definitionsS.
 
-  Context {A B C D: Type} {Σ : gFunctors} {eqa: EqDecision A} {count: Countable A}
+  (* A now needs to be comparable, so we can distinquish between higher and lower a's *)
+  Context {A B C D: Type} {Σ : gFunctors} {eqa: EqDecision A} {a_compare : Ord A}
+          {count: Countable A}
           {sts_std: STS_STD B} {eqc : EqDecision C} {countC: Countable C}
           {eqd : EqDecision D} {countD: Countable D} {stsg : STSG A B Σ}.
   Notation STS := (leibnizO (STS_states * STS_rels)).
@@ -74,8 +84,8 @@ Section definitionsS.
   Definition convert_rel {D : Type} `{Countable D} (R : D → D → Prop) : positive → positive → Prop :=
     λ x y, ∃ a b, x = encode a ∧ y = encode b ∧ R a b.
 
-  Definition sts_rel_loc (i : positive) (R : D → D → Prop) (P : D → D → Prop) : iProp Σ :=
-    own (γr_loc (A:=A)) (◯ {[ i := to_agree ((convert_rel R,convert_rel P)) ]}).
+  Definition sts_rel_loc (i : positive) (R : D → D → Prop) (P : D → D → Prop) (Q : D → D → Prop) : iProp Σ :=
+    own (γr_loc (A:=A)) (◯ {[ i := to_agree ((convert_rel R,convert_rel P,convert_rel Q)) ]}).
 
   Program Definition sts_full γs γr (fs : STS_states) (fr : STS_rels) : iProp Σ
     := (own (A := sts_stateUR) γs (● (Excl <$> fs))
@@ -85,40 +95,77 @@ Section definitionsS.
   Program Definition sts_full_world W : iProp Σ :=
     ((sts_full_std (γs_std (A:=A)) W.1) ∗ (sts_full (γs_loc (A:=A)) (γr_loc (A:=A)) W.2.1 W.2.2))%I.
 
+  (* We will have three kinds of future world relation (here in subset order) :
+     - public
+     - public +
+     - private
+
+     Additionally, we define a special public future world relation that allows
+     public + transitions above an address a, but only public transitions below
+     a
+   *)
+
   Definition related_sts_std_pub (fs gs : STS_std_states A B) : Prop :=
     dom (gset A) fs ⊆ dom (gset A) gs ∧
     ∀ i x y, fs !! i = Some x → gs !! i = Some y → rtc (Rpub) x y.
 
+  Definition related_sts_std_pub_plus (fs gs : STS_std_states A B) : Prop :=
+    dom (gset A) fs ⊆ dom (gset A) gs ∧
+    ∀ i x y, fs !! i = Some x → gs !! i = Some y → rtc (λ x y, (Rpub x y ∨ Rpubp x y)) x y.
+
   Definition related_sts_std_priv (fs gs : STS_std_states A B) : Prop :=
     dom (gset A) fs ⊆ dom (gset A) gs ∧
-    ∀ i x y, fs !! i = Some x → gs !! i = Some y → rtc (λ x y, (Rpub x y ∨ Rpriv x y)) x y.
+    ∀ i x y, fs !! i = Some x → gs !! i = Some y → rtc (λ x y, (Rpub x y ∨ Rpubp x y ∨ Rpriv x y)) x y.
+
+  Program Definition related_sts_a (fs gs : STS_std_states A B) (a : A) : Prop :=
+    dom (gset A) fs ⊆ dom (gset A) gs ∧
+    ∀ (i : A) (x y : B), fs !! i = Some x → gs !! i = Some y →
+                         rtc (λ x y, if (decide(Decision:=le_a_decision i a) (le_a i a))
+                                     then (Rpub x y)
+                                     else (Rpub x y ∨ Rpubp x y)) x y.
 
   Definition related_sts_pub (fs gs : STS_states) (fr gr : STS_rels) : Prop :=
     dom (gset positive) fs ⊆ dom (gset positive) gs ∧
     dom (gset positive) fr ⊆ dom (gset positive) gr ∧
-    ∀ i r1 r2 r1' r2', fr !! i = Some (r1,r2) → gr !! i = Some (r1',r2') →
-                       r1 = r1' ∧ r2 = r2' ∧
-                       (∀ x y, fs !! i = Some x → gs !! i = Some y → rtc r1 x y).
+    ∀ i (r1 r2 r1' r2' r3 r3' : positive → positive → Prop), fr !! i = Some (r1,r2,r3) → gr !! i = Some (r1',r2',r3') →
+                       r1 = r1' ∧ r2 = r2' ∧ r3 = r3' ∧
+                       (∀ x y, fs !! i = Some x → gs !! i = Some y → (rtc r1 x y)).
+
+
+  Definition related_sts_pub_plus (fs gs : STS_states) (fr gr : STS_rels) : Prop :=
+    dom (gset positive) fs ⊆ dom (gset positive) gs ∧
+    dom (gset positive) fr ⊆ dom (gset positive) gr ∧
+    ∀ i (r1 r2 r1' r2' r3 r3' : positive → positive → Prop), fr !! i = Some (r1,r2,r3) → gr !! i = Some (r1',r2',r3') →
+                       r1 = r1' ∧ r2 = r2' ∧ r3 = r3' ∧
+                       (∀ x y, fs !! i = Some x → gs !! i = Some y → (rtc (λ x y, r1 x y ∨ r2 x y) x y)).
 
   Definition related_sts_priv (fs gs : STS_states) (fr gr : STS_rels) : Prop :=
     dom (gset positive) fs ⊆ dom (gset positive) gs ∧
     dom (gset positive) fr ⊆ dom (gset positive) gr ∧
-    ∀ i r1 r2 r1' r2', fr !! i = Some (r1,r2) → gr !! i = Some (r1',r2') →
-                       r1 = r1' ∧ r2 = r2' ∧
-                       (∀ x y, fs !! i = Some x → gs !! i = Some y → (rtc (λ x y, (r1 x y ∨ r2 x y)) x y)).
+    ∀ i (r1 r2 r1' r2' r3 r3' : positive → positive → Prop), fr !! i = Some (r1,r2,r3) → gr !! i = Some (r1',r2',r3') →
+                       r1 = r1' ∧ r2 = r2' ∧ r3 = r3' ∧
+                       (∀ x y, fs !! i = Some x → gs !! i = Some y → (rtc (λ x y, (r1 x y ∨ r2 x y ∨ r3 x y)) x y)).
 
   Definition related_sts_pub_world W W' :=
     related_sts_std_pub W.1 W'.1 ∧
     related_sts_pub W.2.1 W'.2.1 W.2.2 W'.2.2.
 
+  Definition related_sts_pub_plus_world W W' :=
+    related_sts_std_pub_plus W.1 W'.1 ∧
+    related_sts_pub_plus W.2.1 W'.2.1 W.2.2 W'.2.2.
+
   Definition related_sts_priv_world W W' :=
     related_sts_std_priv W.1 W'.1 ∧
     related_sts_priv W.2.1 W'.2.1 W.2.2 W'.2.2.
 
-  Global Instance sts_rel_loc_Persistent i R P : Persistent (sts_rel_loc i R P).
+  Definition related_sts_a_world W W' a :=
+    related_sts_a W.1 W'.1 a ∧
+    related_sts_pub_plus W.2.1 W'.2.1 W.2.2 W'.2.2. 
+
+  Global Instance sts_rel_loc_Persistent i R P Q : Persistent (sts_rel_loc i R P Q).
   Proof. apply _. Qed.
 
-  Global Instance sts_rel_loc_Timeless i R P : Timeless (sts_rel_loc i R P).
+  Global Instance sts_rel_loc_Timeless i R P Q : Timeless (sts_rel_loc i R P Q).
   Proof. apply _. Qed.
 
   Global Instance sts_state_std_Timeless i x : Timeless (sts_state_std i x).
@@ -149,7 +196,8 @@ Proof.
 Qed.
 
 Section pre_STS.
-  Context {A B C D: Type} {Σ : gFunctors} {eqa: EqDecision A} {count: Countable A}
+  Context {A B C D: Type} {Σ : gFunctors} {eqa: EqDecision A} {compare_a: Ord A}
+          {count: Countable A}
           {sts_std: STS_STD B} {eqc : EqDecision C} {countC: Countable C}
           {eqd : EqDecision D} {countD: Countable D} {sts_preg: STS_preG A B Σ}.
 
@@ -171,7 +219,8 @@ Section pre_STS.
 End pre_STS.
 
 Section STS.
-  Context {A B C D: Type} {Σ : gFunctors} {eqa: EqDecision A} {count: Countable A}
+  Context {A B C D: Type} {Σ : gFunctors} {eqa: EqDecision A} {compare_a: Ord A}
+          {count: Countable A}
           {sts_std: STS_STD B} {eqc : EqDecision C} {countC: Countable C}
           {eqd : EqDecision D} {countD: Countable D} {stsg : STSG A B Σ}.
   Implicit Types x y : positive.
@@ -191,11 +240,21 @@ Section STS.
   Notation WORLD := (prodO STS_STD STS).
   Implicit Types W : WORLD.
 
+  (* --------------------- REFLEXIVITY --------------------- *)
+
   Lemma related_sts_pub_refl fs fr : related_sts_pub fs fs fr fr.
   Proof.
     split; [|split]; trivial.
     intros; simplify_eq.
+    split; [|split]; [..|split]; trivial.
+    intros; simplify_eq; eauto using rtc_refl.
+  Qed.
+
+  Lemma related_sts_pub_plus_refl fs fr : related_sts_pub_plus fs fs fr fr.
+  Proof.
     split; [|split]; trivial.
+    intros; simplify_eq.
+    split; [|split]; [..|split]; trivial.
     intros; simplify_eq; eauto using rtc_refl.
   Qed.
 
@@ -203,12 +262,19 @@ Section STS.
   Proof.
     split; [|split]; trivial.
     intros; simplify_eq.
-    split; [|split]; trivial.
+    split; [|split]; [..|split]; trivial.
     intros; simplify_eq;
     eauto using rtc_refl.
   Qed.
 
   Lemma related_sts_std_pub_refl fsd : related_sts_std_pub fsd fsd.
+  Proof.
+    split; trivial.
+    intros; simplify_eq.
+    eauto using rtc_refl.
+  Qed.
+
+  Lemma related_sts_std_pub_plus_refl fsd : related_sts_std_pub_plus fsd fsd.
   Proof.
     split; trivial.
     intros; simplify_eq.
@@ -224,16 +290,21 @@ Section STS.
 
   Lemma related_sts_pub_refl_world W : related_sts_pub_world W W.
   Proof. split;[apply related_sts_std_pub_refl|apply related_sts_pub_refl]. Qed.
+  Lemma related_sts_pub_plus_refl_world W : related_sts_pub_plus_world W W.
+  Proof. split;[apply related_sts_std_pub_plus_refl|apply related_sts_pub_plus_refl]. Qed.
   Lemma related_sts_priv_refl_world W : related_sts_priv_world W W.
   Proof. split;[apply related_sts_std_priv_refl|apply related_sts_priv_refl]. Qed.
 
-  Lemma related_sts_pub_priv fs fr gs gr :
-    related_sts_pub fs gs fr gr → related_sts_priv fs gs fr gr.
+
+  (* --------------------- pub ⊆ pub+ ⊆ priv  --------------------- *)
+
+  Lemma related_sts_pub_pub_plus fs fr gs gr :
+    related_sts_pub fs gs fr gr → related_sts_pub_plus fs gs fr gr.
   Proof.
     rewrite /related_sts_pub /related_sts_priv.
     intros [Hf1 [Hf2 Hf3]].
     do 2 (split; auto). intros.
-    specialize (Hf3 i r1 r2 r1' r2' H H0) as (Hr1 & Hr2 & Hrtc); auto.
+    specialize (Hf3 i r1 r2 r1' r2' r3 r3' H H0) as (Hr1 & Hr2 & Hr3 & Hrtc); auto.
     subst. repeat (split;auto). intros.
     specialize (Hrtc x y H1 H2).
     inversion Hrtc.
@@ -242,30 +313,158 @@ Section STS.
       apply rtc_or_intro. apply H4.
   Qed.
 
+  Lemma related_sts_pub_plus_priv fs fr gs gr :
+    related_sts_pub_plus fs gs fr gr → related_sts_priv fs gs fr gr.
+  Proof.
+    intros [Hf1 [Hf2 Hf3]].
+    do 2 (split; auto). intros.
+    specialize (Hf3 i r1 r2 r1' r2' r3 r3' H H0) as (Hr1 & Hr2 & Hr3 & Hrtc); auto.
+    subst. repeat (split;auto). intros.
+    specialize (Hrtc x y H1 H2).
+    inversion Hrtc.
+    - left.
+    - inversion H3.
+      + right with y0; auto.
+        apply rtc_implies with (R:=(λ x1 y1, (r1' x1 y1 ∨ r2' x1 y1) ∨ r3' x1 y1));
+          [intros ? ? [[?|?]|?];auto|].
+        apply rtc_or_intro;auto.
+      + right with y0; auto.
+        apply rtc_implies with (R:=(λ x1 y1, (r1' x1 y1 ∨ r2' x1 y1) ∨ r3' x1 y1));
+          [intros ? ? [[?|?]|?];auto|].
+        apply rtc_or_intro;auto.
+  Qed.
+
+  Lemma related_sts_pub_priv fs fr gs gr :
+    related_sts_pub fs gs fr gr → related_sts_priv fs gs fr gr.
+  Proof.
+    intros Hpub.
+    by apply related_sts_pub_plus_priv, related_sts_pub_pub_plus.
+  Qed.
+
+  Lemma related_sts_std_pub_pub_plus fsd gsd :
+    related_sts_std_pub fsd gsd → related_sts_std_pub_plus fsd gsd.
+  Proof.
+    intros [Hf1 Hf2].
+    split;auto. intros i x y Hx Hy.
+    specialize (Hf2 i x y Hx Hy).
+    apply rtc_or_intro. auto.
+  Qed.
+
+  Lemma related_sts_std_pub_plus_priv fsd gsd :
+    related_sts_std_pub_plus fsd gsd → related_sts_std_priv fsd gsd.
+  Proof.
+    intros [Hf1 Hf2].
+    split;auto. intros i x y Hx Hy.
+    specialize (Hf2 i x y Hx Hy).
+    eapply rtc_implies;[|eauto].
+    intros r q [Hr | Hq];auto.
+  Qed.
+
   Lemma related_sts_std_pub_priv fsd gsd :
     related_sts_std_pub fsd gsd → related_sts_std_priv fsd gsd.
   Proof.
-    rewrite /related_sts_pub /related_sts_priv.
-    intros [Hf1 Hf2].
-    repeat (split; auto). intros.
-    specialize (Hf2 i _ _ H H0) as Hrtc; auto.
-    inversion Hrtc.
-    - left.
-    - right with y0; auto.
-      apply rtc_or_intro. subst. auto.
+    intros Hpub. by apply related_sts_std_pub_plus_priv, related_sts_std_pub_pub_plus.
   Qed.
+
+  Lemma related_sts_pub_pub_plus_world W W' :
+    related_sts_pub_world W W' → related_sts_pub_plus_world W W'.
+  Proof.
+    intros [Hrel Hrel'].
+    split;[apply related_sts_std_pub_pub_plus|apply related_sts_pub_pub_plus];auto.
+  Qed.
+  Lemma related_sts_pub_plus_priv_world W W' :
+    related_sts_pub_plus_world W W' → related_sts_priv_world W W'.
+  Proof.
+    intros [Hrel Hrel'].
+    split;[apply related_sts_std_pub_plus_priv|apply related_sts_pub_plus_priv];auto.
+  Qed.
+  Lemma related_sts_pub_priv_world W W' :
+    related_sts_pub_world W W' → related_sts_priv_world W W'.
+  Proof.
+    intros [Hrel Hrel'].
+    split;[apply related_sts_std_pub_priv|apply related_sts_pub_priv];auto.
+  Qed. 
+
+  (* --------------------- pub a lemmas --------------------- *)
+
+  Lemma related_sts_a_weak fsd gsd a a' :
+    le_a a' a →
+    related_sts_a fsd gsd a → related_sts_a fsd gsd a'.
+  Proof.
+    intros Hleb [Hdom Ha].
+    split;auto. intros i x y Hx Hy.
+    specialize (Ha i x y Hx Hy).
+    eapply rtc_implies;[|eauto].
+    intros r q Hr.
+    destruct (decide (le_a i a')).
+    - assert (le_a i a) as Hle.
+      { assert (Transitive le_a) as Htrans;[eapply PreOrder_Transitive|trans a';auto]. }
+      rewrite decide_True in Hr;auto.
+    - destruct (decide (le_a i a));auto.
+      Unshelve. apply le_a_preorder.
+  Qed.
+
+  Lemma related_sts_a_weak_world W W' a a' :
+    le_a a' a →
+    related_sts_a_world W W' a → related_sts_a_world W W' a'.
+  Proof.
+    destruct W,W'.
+    intros Hle [Hrel Hrel']. split; simpl in *.
+    - by pose proof (related_sts_a_weak _ _ _ _ Hle Hrel).
+    - auto.
+  Qed.
+
+  Lemma related_sts_a_pub_plus fsd gsd a :
+    related_sts_a fsd gsd a → related_sts_std_pub_plus fsd gsd.
+  Proof.
+    intros [Hdom Hrel]. split;auto.
+    intros i x y Hx Hy.
+    specialize (Hrel i x y Hx Hy).
+    destruct (decide (le_a i a)).
+    - apply rtc_or_intro. auto.
+    - auto.
+  Qed.
+
+  Lemma related_sts_pub_a fsd gsd a :
+    related_sts_std_pub fsd gsd → related_sts_a fsd gsd a.
+  Proof.
+    intros [Hdom Hrel].
+    split;auto. intros i x y Hx Hy.
+    specialize (Hrel i x y Hx Hy).
+    destruct (decide (le_a i a)).
+    - auto.
+    - apply rtc_or_intro. auto.
+  Qed. 
+
+  Lemma related_sts_a_pub_plus_world W W' a :
+    related_sts_a_world W W' a → related_sts_pub_plus_world W W'.
+  Proof.
+    intros [Hrel Hrel'].
+    apply related_sts_a_pub_plus in Hrel.
+    split;auto.
+  Qed.
+
+  Lemma related_sts_pub_a_world W W' a :
+    related_sts_pub_world W W' → related_sts_a_world W W' a.
+  Proof.
+    intros [Hrel Hrel']. split.
+    - apply related_sts_pub_a. auto.
+    - apply related_sts_pub_pub_plus. auto.
+  Qed.
+
+  (* --------------------- TRANSITIVITY --------------------- *)
 
   Lemma related_sts_pub_trans fs fr gs gr hs hr :
     related_sts_pub fs gs fr gr → related_sts_pub gs hs gr hr →
     related_sts_pub fs hs fr hr.
   Proof.
     intros [Hf1 [Hf2 Hf3]] [Hg1 [Hg2 Hg3]]; split; [|split]; try by etrans.
-    intros i r1 r2 r1' r2' Hfr Hhr.
+    intros i r1 r2 r1' r2' r3 r3' Hfr Hhr.
     specialize (Hf1 i); specialize (Hf2 i);
       revert Hf1 Hf2; rewrite !elem_of_dom; intros Hf1 Hf2.
-    destruct Hf2; eauto. destruct x as [x1 x2].
-    edestruct Hf3 as [Heq1 [Heq2 Hrtc] ] ; eauto; simplify_eq.
-    edestruct Hg3 as [Heq1 [Heq2 Hrtc'] ] ; eauto; simplify_eq.
+    destruct Hf2; eauto. destruct x as [[x1 x2] x3].
+    edestruct Hf3 as [Heq1 [Heq2 [Heq3 Hrtc]] ] ; eauto; simplify_eq.
+    edestruct Hg3 as [Heq1 [Heq2 [Heq3 Hrtc']] ] ; eauto; simplify_eq.
     repeat (split;auto).
     intros x y Hx Hy.
     destruct Hf1;eauto.
@@ -291,12 +490,12 @@ Section STS.
     related_sts_priv fs hs fr hr.
   Proof.
     intros [Hf1 [Hf2 Hf3]] [Hg1 [Hg2 Hg3]]; split; [|split]; try by etrans.
-    intros i r1 r2 r1' r2' Hfr Hhr.
+    intros i r1 r2 r1' r2' r3 r3' Hfr Hhr.
     specialize (Hf1 i); specialize (Hf2 i);
       revert Hf1 Hf2; rewrite !elem_of_dom; intros Hf1 Hf2.
-    destruct Hf2; eauto. destruct x as [x1 x2].
-    edestruct Hf3 as [Heq1 [Heq2 Hrtc] ] ; eauto; simplify_eq.
-    edestruct Hg3 as [Heq1 [Heq2 Hrtc'] ] ; eauto; simplify_eq.
+    destruct Hf2; eauto. destruct x as [[x1 x2] x3].
+    edestruct Hf3 as [Heq1 [Heq2 [Heq3 Hrtc]] ] ; eauto; simplify_eq.
+    edestruct Hg3 as [Heq1 [Heq2 [Heq3 Hrtc']] ] ; eauto; simplify_eq.
     repeat (split;auto).
     intros x y Hx Hy.
     destruct Hf1;eauto.
@@ -324,12 +523,12 @@ Section STS.
     related_sts_priv fs hs fr hr.
   Proof.
     intros [Hf1 [Hf2 Hf3]] [Hg1 [Hg2 Hg3]]; split; [|split]; try by etrans.
-    intros i r1 r2 r1' r2' Hfr Hhr.
+    intros i r1 r2 r1' r2' r3 r3' Hfr Hhr.
     specialize (Hf1 i); specialize (Hf2 i);
       revert Hf1 Hf2; rewrite !elem_of_dom; intros Hf1 Hf2.
-    destruct Hf2; eauto. destruct x as [x1 x2].
-    edestruct Hf3 as [Heq1 [Heq2 Hrtc] ] ; eauto; simplify_eq.
-    edestruct Hg3 as [Heq1 [Heq2 Hrtc'] ] ; eauto; simplify_eq.
+    destruct Hf2; eauto. destruct x as [[x1 x2] x3].
+    edestruct Hf3 as [Heq1 [Heq2 [Heq3 Hrtc]] ] ; eauto; simplify_eq.
+    edestruct Hg3 as [Heq1 [Heq2 [Heq3 Hrtc']] ] ; eauto; simplify_eq.
     repeat (split;auto).
     intros x y Hx Hy.
     destruct Hf1;eauto.
@@ -357,12 +556,12 @@ Section STS.
     related_sts_priv fs hs fr hr.
   Proof.
     intros [Hf1 [Hf2 Hf3]] [Hg1 [Hg2 Hg3]]; split; [|split]; try by etrans.
-    intros i r1 r2 r1' r2' Hfr Hhr.
+    intros i r1 r2 r1' r2' r3 r3' Hfr Hhr.
     specialize (Hf1 i); specialize (Hf2 i);
       revert Hf1 Hf2; rewrite !elem_of_dom; intros Hf1 Hf2.
-    destruct Hf2; eauto. destruct x as [x1 x2].
-    edestruct Hf3 as [Heq1 [Heq2 Hrtc] ] ; eauto; simplify_eq.
-    edestruct Hg3 as [Heq1 [Heq2 Hrtc'] ] ; eauto; simplify_eq.
+    destruct Hf2; eauto. destruct x as [[x1 x2] x3].
+    edestruct Hf3 as [Heq1 [Heq2 [Heq3 Hrtc]] ] ; eauto; simplify_eq.
+    edestruct Hg3 as [Heq1 [Heq2 [Heq3 Hrtc']] ] ; eauto; simplify_eq.
     repeat (split;auto).
     intros x y Hx Hy.
     destruct Hf1;eauto.
@@ -374,6 +573,42 @@ Section STS.
     related_sts_std_priv fsd hsd.
   Proof.
     intros [Hf1 Hf2] [Hg1 Hg2]; split; try by etrans.
+    intros i x y Hx Hy.
+    specialize (Hf1 i);
+      revert Hf1; rewrite !elem_of_dom; intros Hf1.
+    destruct Hf1 as [x0 Hx0]; eauto.
+    specialize (Hf2 i x x0 Hx Hx0); simplify_eq.
+    specialize (Hg2 i x0 y Hx0 Hy); simplify_eq.
+    etrans;eauto.
+  Qed.
+
+  Lemma related_sts_a_trans_left fsd gsd hsd a a' :
+    le_a a a' →
+    related_sts_a fsd gsd a → related_sts_a gsd hsd a' →
+    related_sts_a fsd hsd a.
+  Proof.
+    intros Hle Hrel1 Hrel2.
+    apply related_sts_a_weak with (a':=a) in Hrel2;[|auto].
+    destruct Hrel1 as [Hf1 Hf2]; destruct Hrel2 as [Hg1 Hg2].
+    split; try by etrans.
+    intros i x y Hx Hy.
+    specialize (Hf1 i);
+      revert Hf1; rewrite !elem_of_dom; intros Hf1.
+    destruct Hf1 as [x0 Hx0]; eauto.
+    specialize (Hf2 i x x0 Hx Hx0); simplify_eq.
+    specialize (Hg2 i x0 y Hx0 Hy); simplify_eq.
+    etrans;eauto.
+  Qed.
+
+  Lemma related_sts_a_trans_right fsd gsd hsd a a' :
+    le_a a a' →
+    related_sts_a fsd gsd a' → related_sts_a gsd hsd a →
+    related_sts_a fsd hsd a.
+  Proof.
+    intros Hle Hrel1 Hrel2.
+    apply related_sts_a_weak with (a':=a) in Hrel1;[|auto].
+    destruct Hrel1 as [Hf1 Hf2]; destruct Hrel2 as [Hg1 Hg2].
+    split; try by etrans.
     intros i x y Hx Hy.
     specialize (Hf1 i);
       revert Hf1; rewrite !elem_of_dom; intros Hf1.
@@ -424,12 +659,6 @@ Section STS.
     - apply related_sts_pub_trans with W'.2.1 W'.2.2; auto.
   Qed.
 
-  Lemma related_sts_pub_priv_world W W' :
-    related_sts_pub_world W W' -> related_sts_priv_world W W'.
-  Proof.
-    intros [Hstd Hloc].
-    split; [apply related_sts_std_pub_priv|apply related_sts_pub_priv]; auto.
-  Qed.
 
   Lemma related_sts_priv_world_std_sta_is_Some W W' i :
     related_sts_priv_world W W' -> is_Some ((W.1) !! i) -> is_Some ((W'.1) !! i).
@@ -453,8 +682,9 @@ Section STS.
     eauto.
   Qed.
 
-  Lemma sts_full_rel_loc W i Q P :
-    sts_full_world W -∗ sts_rel_loc (A:=A) i Q P -∗ ⌜W.2.2 !! i = Some (convert_rel Q,convert_rel P)⌝.
+  Lemma sts_full_rel_loc W i Q Q' P :
+    sts_full_world W -∗ sts_rel_loc (A:=A) i Q Q' P  -∗
+                   ⌜W.2.2 !! i = Some (convert_rel Q,convert_rel Q',convert_rel P)⌝.
   Proof.
     rewrite /sts_rel_loc /sts_full_world /sts_full.
     destruct W as [Wstd [fs fr]].
@@ -509,7 +739,7 @@ Section STS.
     apply Some_included_exclusive in HR; auto; last by typeclasses eauto.
     apply leibniz_equiv in HR; simplify_eq; eauto.
   Qed.
-
+ 
   Lemma sts_dealloc_std W a b :
     sts_full_world W ∗ sts_state_std a b ==∗ sts_full_world (delete a W.1,W.2).
   Proof.
@@ -550,11 +780,11 @@ Section STS.
     iFrame. done.
   Qed.
 
-  Lemma sts_alloc_loc W d Q P:
+  Lemma sts_alloc_loc W d Q Q' P:
     sts_full_world W ==∗
-             ∃ i, sts_full_world (W.1,((<[i := encode d ]>W.2.1),(<[i := (convert_rel Q,convert_rel P) ]>W.2.2)))
+             ∃ i, sts_full_world (W.1,((<[i := encode d ]>W.2.1),(<[i := (convert_rel Q,convert_rel Q',convert_rel P) ]>W.2.2)))
                   ∗ ⌜i ∉ dom (gset positive) W.2.1⌝ ∗ ⌜i ∉ dom (gset positive) W.2.2⌝
-                  ∗ sts_state_loc (A:=A) i d ∗ sts_rel_loc (A:=A) i Q P.
+                  ∗ sts_state_loc (A:=A) i d ∗ sts_rel_loc (A:=A) i Q Q' P.
   Proof.
     rewrite /sts_full_world /sts_full /sts_rel_loc /sts_state_loc.
     (* iIntros "[Hd [H1 H2]]". *)
@@ -582,8 +812,8 @@ Section STS.
             (A := sts_relUR)
             _ _
             (● (to_agree <$>
-                <[fresh (dom (gset positive) fs ∪ dom (gset positive) fr) := (convert_rel Q,convert_rel P)]> fr)
-            ⋅ ◯ {[fresh (dom (gset positive) fs ∪ dom (gset positive) fr) := to_agree (convert_rel Q,convert_rel P)]})
+                <[fresh (dom (gset positive) fs ∪ dom (gset positive) fr) := (convert_rel Q,convert_rel Q',convert_rel P)]> fr)
+            ⋅ ◯ {[fresh (dom (gset positive) fs ∪ dom (gset positive) fr) := to_agree (convert_rel Q,convert_rel Q',convert_rel P)]})
             with "H2") as "[H2 Hr]".
     { apply auth_update_alloc.
       rewrite fmap_insert /=.
